Weidenbach_Book/CDCL_Two_Watched_Literals_Code_Common.thy
@@ -110,7 +110,7 @@ sepref_decl_op lit_of: "lit_of :: (nat, nat) ann_lit \<Rightarrow> nat literal" 
 lemma [def_pat_rules]:
   "lit_of \<equiv> op_lit_of"
   by auto
-  
+
 sepref_decl_op option_bool_eq: "op = :: bool option \<Rightarrow> bool option \<Rightarrow> bool" ::
   "(Id :: ((bool option \<times> _) set)) \<rightarrow> (Id :: (bool option \<times> _) set) \<rightarrow> (Id :: (bool \<times> _) set)" .
 
